add more bruteforce tools...

Libs/Logic_extended.v
@@ -1,6 +1,8 @@
 From Tweetnacl Require Export Libs.LibTactics.
+From Tweetnacl Require Export Libs.LibTactics_SF.
 Require Import Coq.micromega.Lia.
 Require Import ssreflect.
+Require Import Recdef.
 
 Lemma orFalse : forall (P:Prop), P \/ False <-> P.
 Proof. boum. Qed.
@@ -18,6 +20,7 @@ Fixpoint forall_nat (i:nat) (P:nat -> bool) := match i with
   | 0 => true
   | S n => andb (P n) (forall_nat n P)
   end.
+
 
 Lemma forall_nat_refl : forall (P: nat -> bool) (n: nat),
   (forall i, 0 <= i < n -> P i = true) <-> forall_nat n P = true.
@@ -51,6 +54,218 @@ go.
 Qed.
 
 Open Scope Z.
+
+Section fun_bool_rec.
+
+(* Context (n_min:Z). (* (Hn : 0 <= n). *) *)
+
+Definition dec_proof_fun (n_min a  : Z) : nat := Z.to_nat (a - n_min).
+
+Function forall_Z (n_min:Z) (a:Z) (P:Z -> bool) {measure (dec_proof_fun n_min) a} : bool :=
+  if (a <=? n_min)
+    then true
+    else
+      andb (P (a - 1)) (forall_Z n_min (a - 1) P).
+Proof. intros. apply Z2Nat.inj_lt; apply Z.leb_gt in teq; omega. Defined.
+
+(* Lemma forall_Z_translate: forall n_min n_max P,
+  n_min <= n_max ->
+  forall_Z n_min n_max P = forall_Z 0 (n_max - n_min) (fun x => P (x + n_min)).
+Proof.
+intros.
+assert(exists n, (n_max - n_min) = Z.of_nat n).
+apply Z_of_nat_complete; omega.
+destruct H0 as [n Hn].
+revert Hn.
+revert H.
+revert n_min n_max.
+induction n ; intros.
+revert Hn. change_Z_of_nat => Hn.
+assert(n_max = n_min) by omega.
+subst.
+rewrite Hn.
+rewrite forall_Z_equation. symmetry. rewrite forall_Z_equation.
+rewrite ?Zle_imp_le_bool.
+omega.
+omega.
+reflexivity.
+rewrite Nat2Z.inj_succ in Hn.
+change (Z.succ ?A) with (A + 1) in Hn.
+assert(n_max = n_min + Z.of_nat n + 1).
+omega.
+rewrite forall_Z_equation. symmetry. rewrite forall_Z_equation.
+replace (n_max - n_min <=? 0) with false.
+2: symmetry ; apply Z.leb_gt ; omega.
+replace (n_max <=? n_min) with false.
+2: symmetry ; apply Z.leb_gt ; omega.
+fequals.
+fequals.
+omega.
+symmetry.
+assert(n_max - n_min - 1 = Z.of_nat n).
+omega.
+replace (n_max - n_min - 1) with (n_max - 1 - n_min).
+2: omega.
+apply IHn ; omega.
+Qed.
+ *)
+Lemma forall_Z_refl : forall (P: Z -> bool) (n_min n_max: Z),
+  (forall i, n_min <= i < n_max -> P i = true) <-> forall_Z n_min n_max P = true.
+Proof.
+intros P n_min n_max.
+assert(n_max <= n_min \/ n_min <= n_max).
+omega.
+destruct H as [Hminmax|Hminmax] ; split ; intros; try omega.
+rewrite forall_Z_equation.
+rewrite Zle_imp_le_bool.
+omega.
+reflexivity.
+(* -> *)
+assert(Hn: exists n, (n_max - n_min) = Z.of_nat n).
+apply Z_of_nat_complete; omega.
+destruct Hn as [n Hn].
+revert H.
+revert Hn.
+revert Hminmax.
+revert n_min n_max.
+induction n ; intros.
+revert Hn. change_Z_of_nat => Hn.
+assert(n_max = n_min) by omega.
+rewrite forall_Z_equation.
+rewrite ?Zle_imp_le_bool.
+omega.
+reflexivity.
+rewrite Nat2Z.inj_succ in Hn.
+change (Z.succ ?A) with (A + 1) in Hn.
+assert(n_max = n_min + Z.of_nat n + 1).
+omega.
+rewrite forall_Z_equation.
+replace (n_max <=? n_min) with false.
+2: symmetry ; apply Z.leb_gt ; omega.
+apply andb_true_iff ; split.
+apply H.
+omega.
+apply IHn.
+omega.
+omega.
+intros ; apply H ; omega.
+(* <- *)
+assert(Hn: exists n, (n_max - n_min) = Z.of_nat n).
+apply Z_of_nat_complete; omega.
+destruct Hn as [n Hn].
+revert H.
+revert H0.
+revert Hn.
+revert Hminmax.
+revert n_min n_max i.
+induction n ; intros.
+revert Hn. change_Z_of_nat => Hn.
+omega.
+rewrite Nat2Z.inj_succ in Hn.
+change (Z.succ ?A) with (A + 1) in Hn.
+assert(n_max = n_min + Z.of_nat n + 1).
+omega.
+rewrite forall_Z_equation in H.
+replace (n_max <=? n_min) with false in H.
+2: symmetry ; apply Z.leb_gt ; omega.
+apply andb_true_iff in H ; destruct H as [Hi Hi1].
+assert(i < n_max - 1 \/ i = n_max - 1).
+omega.
+destruct H.
+2: rewrite H ; assumption.
+eapply IHn.
+4: apply Hi1.
+omega.
+omega.
+omega.
+Qed.
+
+Function forall_Z_Z (m_min:Z) (m_max:Z) (n_min:Z) (a:Z) (P:Z -> Z -> bool)
+  {measure (dec_proof_fun n_min) a} : bool :=
+  if (a <=? n_min)
+    then true
+    else
+      andb (forall_Z m_min m_max (P (a - 1))) (forall_Z_Z m_min m_max n_min (a - 1) P).
+Proof. intros; apply Z2Nat.inj_lt; apply Z.leb_gt in teq; omega. Defined.
+
+Lemma forall_Z_Z_refl : forall (P: Z -> Z -> bool) (m_min m_max: Z) (n_min n_max: Z),
+  (forall i j, n_min <= i < n_max -> m_min <= j < m_max -> P i j = true) <-> forall_Z_Z m_min m_max n_min n_max P = true.
+Proof.
+intros P m_min m_max n_min n_max.
+assert(n_max <= n_min \/ n_min <= n_max).
+omega.
+destruct H as [Hminmax|Hminmax] ; split ; intros; try omega.
+rewrite forall_Z_Z_equation.
+rewrite Zle_imp_le_bool.
+omega.
+reflexivity.
+(* -> *)
+assert(Hn: exists n, (n_max - n_min) = Z.of_nat n).
+apply Z_of_nat_complete; omega.
+destruct Hn as [n Hn].
+revert H.
+revert Hn.
+revert Hminmax.
+revert m_min m_max.
+revert n_min n_max.
+induction n ; intros.
+revert Hn. change_Z_of_nat => Hn.
+assert(n_max = n_min) by omega.
+rewrite forall_Z_Z_equation.
+rewrite ?Zle_imp_le_bool.
+omega.
+reflexivity.
+
+rewrite Nat2Z.inj_succ in Hn.
+change (Z.succ ?A) with (A + 1) in Hn.
+assert(n_max = n_min + Z.of_nat n + 1).
+omega.
+rewrite forall_Z_Z_equation.
+replace (n_max <=? n_min) with false.
+2: symmetry ; apply Z.leb_gt ; omega.
+apply andb_true_iff ; split.
+apply forall_Z_refl ; intros.
+apply H ; omega.
+apply IHn ; try omega.
+intros ; apply H ; omega.
+
+(* <- *)
+assert(Hn: exists n, (n_max - n_min) = Z.of_nat n).
+apply Z_of_nat_complete; omega.
+destruct Hn as [n Hn].
+revert H.
+revert H0.
+revert H1.
+revert Hn.
+revert Hminmax.
+revert m_min m_max.
+revert n_min n_max i.
+induction n ; intros.
+revert Hn. change_Z_of_nat => Hn.
+omega.
+rewrite Nat2Z.inj_succ in Hn.
+change (Z.succ ?A) with (A + 1) in Hn.
+assert(n_max = n_min + Z.of_nat n + 1).
+omega.
+rewrite forall_Z_Z_equation in H.
+replace (n_max <=? n_min) with false in H.
+2: symmetry ; apply Z.leb_gt ; omega.
+apply andb_true_iff in H ; destruct H as [Hi Hi1].
+assert(i < n_max - 1 \/ i = n_max - 1).
+omega.
+destruct H.
+eapply IHn.
+5: apply Hi1.
+all : try omega.
+subst i.
+assert(Hnn:=forall_Z_refl (P (n_max - 1)) m_min m_max).
+apply Hnn.
+assumption.
+omega.
+Qed.
+
+End fun_bool_rec.
+
 
 (* Ltac gen_goals H P j n := match n with 
   | 0 => idtac
