Low/M_low_level_compute.v
@@ -9,7 +9,6 @@ Local Open Scope Z.
 simpl ; unfold update_M_i_j' ; unfold local_update_M ;reflexivity. *)
 Ltac inner_M_fix_compute_solve := intros ; repeat orewrite inner_M_i_j_eq ; simpl ; unfold update_M_i_j' ; unfold local_update_M ;reflexivity.
 
-
 Lemma inner_M_fix_0_16 : forall z0 z15 z16 z17 z18 z19 z20 z21 z22 z23 z24 z25 z26 z27 z28 z29
   z30 z31 z32 z33 z34 z35 z36 z37 z38 z39 z40 z41 z42 z43 z44 z45 z46 z47 z48 z49 z50 z51 z52 z53 z54 z55 z56 z57 z58 z59 z60 z61,
   (inner_M_fix 0 16 z0
@@ -23,7 +22,7 @@ z0 * z19 + z35; z0 * z20 + z36; z0 * z21 + z37; z0 * z22 + z38;
 z0 * z23 + z39; z0 * z24 + z40; z0 * z25 + z41; z0 * z26 + z42;
 z0 * z27 + z43; z0 * z28 + z44; z0 * z29 + z45; z0 * z30 + z46; z47; z48;
 z49; z50; z51; z52; z53; z54; z55; z56; z57; z58; z59; z60; z61].
-Proof.  inner_M_fix_compute_solve. Qed.
+Proof. inner_M_fix_compute_solve. Qed.
 
 Lemma inner_M_fix_1_16 : forall z0 z15 z16 z17 z18 z19 z20 z21 z22 z23 z24 z25 z26 z27 z28 z29
   z30 z31 z32 z33 z34 z35 z36 z37 z38 z39 z40 z41 z42 z43 z44 z45 z46 z47 z48 z49 z50 z51 z52 z53 z54 z55 z56 z57 z58 z59 z60 z61,
